code/sha3/Hacl.Hash.SHA3.Scalar.fst
@@ -1,0 +1,114 @@
+module Hacl.Hash.SHA3.Scalar
+
+open FStar.HyperStack
+open FStar.HyperStack.ST
+open FStar.Mul
+
+open LowStar.Buffer
+
+open Lib.IntTypes
+open Lib.Buffer
+open Lib.ByteBuffer
+
+open Spec.Hash.Definitions
+open Hacl.Spec.SHA3.Vec
+open Hacl.Spec.SHA3.Vec.Common
+open Hacl.Impl.SHA3.Vec
+
+module S = Spec.SHA3
+module ST = FStar.HyperStack.ST
+module B = LowStar.Buffer
+
+#reset-options "--z3rlimit 50 --max_fuel 0 --max_ifuel 0 --using_facts_from '* -FStar.Seq'"
+
+val shake128:
+  output:buffer_t MUT uint8
+  -> outputByteLen:size_t{v outputByteLen == length output}
+  -> input:buffer_t MUT uint8
+  -> inputByteLen:size_t{v inputByteLen == length input}
+  -> Stack unit
+     (requires fun h ->
+       live h input /\ live h output /\ disjoint input output)
+     (ensures  fun h0 _ h1 ->
+       modifies (loc output) h0 h1 /\
+       as_seq h1 (output <: lbuffer uint8 outputByteLen) ==
+       S.shake128 (v inputByteLen) (as_seq h0 (input <: lbuffer uint8 inputByteLen)) (v outputByteLen))
+let shake128 output outputByteLen input inputByteLen =
+  admit();
+  keccak #Shake128 #M32 1344ul (* 256ul *) inputByteLen input (byte 0x1F) outputByteLen output
+
+val shake256:
+  output:buffer_t MUT uint8
+  -> outputByteLen:size_t{v outputByteLen == length output}
+  -> input:buffer_t MUT uint8
+  -> inputByteLen:size_t{v inputByteLen == length input}
+  -> Stack unit
+     (requires fun h ->
+       live h input /\ live h output /\ disjoint input output)
+     (ensures  fun h0 _ h1 ->
+       modifies (loc output) h0 h1 /\
+       as_seq h1 (output <: lbuffer uint8 outputByteLen) ==
+       S.shake256 (v inputByteLen) (as_seq h0 (input <: lbuffer uint8 inputByteLen)) (v outputByteLen))
+let shake256 output outputByteLen input inputByteLen =
+  admit();
+  keccak #Shake256 #M32 1088ul (* 512ul *) inputByteLen input (byte 0x1F) outputByteLen output
+
+val sha3_224:
+  output:lbuffer uint8 28ul
+  -> input:buffer_t MUT uint8
+  -> inputByteLen:size_t{v inputByteLen == length input}
+  -> Stack unit
+     (requires fun h ->
+       live h input /\ live h output /\ disjoint input output)
+     (ensures  fun h0 _ h1 ->
+       modifies (loc output) h0 h1 /\
+       as_seq h1 output ==
+       S.sha3_224 (v inputByteLen) (as_seq h0 (input <: lbuffer uint8 inputByteLen)))
+let sha3_224 output input inputByteLen =
+  admit();
+  keccak #SHA3_224 #M32 1152ul (* 448ul *) inputByteLen input (byte 0x06) 28ul output
+
+val sha3_256:
+  output:lbuffer uint8 32ul
+  -> input:buffer_t MUT uint8
+  -> inputByteLen:size_t{v inputByteLen == length input}
+  -> Stack unit
+     (requires fun h ->
+       live h input /\ live h output /\ disjoint input output)
+     (ensures  fun h0 _ h1 ->
+       modifies (loc output) h0 h1 /\
+       as_seq h1 output ==
+       S.sha3_256 (v inputByteLen) (as_seq h0 (input <: lbuffer uint8 inputByteLen)))
+let sha3_256 output input inputByteLen =
+  admit();
+  keccak #SHA3_256 #M32 1088ul (* 512ul *) inputByteLen input (byte 0x06) 32ul output
+
+val sha3_384:
+  output:lbuffer uint8 48ul
+  -> input:buffer_t MUT uint8
+  -> inputByteLen:size_t{v inputByteLen == length input}
+  -> Stack unit
+     (requires fun h ->
+       live h input /\ live h output /\ disjoint input output)
+     (ensures  fun h0 _ h1 ->
+       modifies (loc output) h0 h1 /\
+       as_seq h1 output ==
+       S.sha3_384 (v inputByteLen) (as_seq h0 (input <: lbuffer uint8 inputByteLen)))
+let sha3_384 output input inputByteLen =
+  admit();
+  keccak #SHA3_384 #M32 832ul (* 768ul *) inputByteLen input (byte 0x06) 48ul output
+
+val sha3_512:
+  output:lbuffer uint8 64ul
+  -> input:buffer_t MUT uint8
+  -> inputByteLen:size_t{v inputByteLen == length input}
+  -> Stack unit
+     (requires fun h ->
+       live h input /\ live h output /\ disjoint input output)
+     (ensures  fun h0 _ h1 ->
+       modifies (loc output) h0 h1 /\
+       as_seq h1 output ==
+       S.sha3_512 (v inputByteLen) (as_seq h0 (input <: lbuffer uint8 inputByteLen)))
+let sha3_512 output input inputByteLen =
+  admit();
+  keccak #SHA3_512 #M32 576ul (* 1024ul *) inputByteLen input (byte 0x06) 64ul output
