code/sha3/Hacl.Hash.SHA3.Simd256.fst
@@ -1,0 +1,256 @@
+module Hacl.Hash.SHA3.Simd256
+
+open FStar.HyperStack
+open FStar.HyperStack.ST
+open FStar.Mul
+
+open LowStar.Buffer
+
+open Lib.IntTypes
+open Lib.NTuple
+open Lib.Buffer
+open Lib.ByteBuffer
+open Lib.MultiBuffer
+
+open Spec.Hash.Definitions
+open Hacl.Spec.SHA3.Vec
+open Hacl.Spec.SHA3.Vec.Common
+open Hacl.Impl.SHA3.Vec
+
+module S = Spec.SHA3
+module ST = FStar.HyperStack.ST
+module B = LowStar.Buffer
+
+#reset-options "--z3rlimit 50 --max_fuel 0 --max_ifuel 0 --using_facts_from '* -FStar.Seq'"
+
+val shake128:
+  output0:buffer_t MUT uint8
+  -> output1:buffer_t MUT uint8
+  -> output2:buffer_t MUT uint8
+  -> output3:buffer_t MUT uint8
+  -> outputByteLen:size_t{v outputByteLen == length output0 /\ 
+                          v outputByteLen == length output1 /\
+                          v outputByteLen == length output2 /\
+                          v outputByteLen == length output3}
+  -> input0:buffer_t MUT uint8
+  -> input1:buffer_t MUT uint8
+  -> input2:buffer_t MUT uint8
+  -> input3:buffer_t MUT uint8
+  -> inputByteLen:size_t{v inputByteLen == length input0 /\ 
+                         v inputByteLen == length input1 /\
+                         v inputByteLen == length input2 /\
+                         v inputByteLen == length input3}
+  -> Stack unit
+     (requires fun h ->
+       live4 h (input0 <: lbuffer uint8 inputByteLen)
+               (input1 <: lbuffer uint8 inputByteLen)
+               (input2 <: lbuffer uint8 inputByteLen)
+               (input3 <: lbuffer uint8 inputByteLen) /\
+       live4 h (output0 <: lbuffer uint8 outputByteLen)
+               (output1 <: lbuffer uint8 outputByteLen)
+               (output2 <: lbuffer uint8 outputByteLen)
+               (output3 <: lbuffer uint8 outputByteLen) /\
+       internally_disjoint4 (output0 <: lbuffer uint8 outputByteLen)
+                            (output1 <: lbuffer uint8 outputByteLen)
+                            (output2 <: lbuffer uint8 outputByteLen)
+                            (output3 <: lbuffer uint8 outputByteLen))
+     (ensures  fun h0 _ h1 ->
+       modifies (loc output0 |+| loc output1 |+| loc output2 |+| loc output3) h0 h1 /\
+       as_seq h1 (output0 <: lbuffer uint8 outputByteLen) ==
+        S.shake128 (v inputByteLen) (as_seq h0 (input0 <: lbuffer uint8 inputByteLen)) (v outputByteLen) /\
+       as_seq h1 (output1 <: lbuffer uint8 outputByteLen) ==
+        S.shake128 (v inputByteLen) (as_seq h0 (input1 <: lbuffer uint8 inputByteLen)) (v outputByteLen) /\
+       as_seq h1 (output2 <: lbuffer uint8 outputByteLen) ==
+        S.shake128 (v inputByteLen) (as_seq h0 (input2 <: lbuffer uint8 inputByteLen)) (v outputByteLen) /\
+       as_seq h1 (output3 <: lbuffer uint8 outputByteLen) ==
+        S.shake128 (v inputByteLen) (as_seq h0 (input3 <: lbuffer uint8 inputByteLen)) (v outputByteLen))
+let shake128 output0 output1 output2 output3 outputByteLen
+      input0 input1 input2 input3 inputByteLen =
+  admit();
+  let ib = ntup4 (input0,(input1,(input2,input3))) in
+  let rb = ntup4 (output0,(output1,(output2,output3))) in
+  keccak #Shake128 #M256 1344ul (* 256ul *) inputByteLen ib (byte 0x1F) outputByteLen rb
+
+val shake256:
+  output0:buffer_t MUT uint8
+  -> output1:buffer_t MUT uint8
+  -> output2:buffer_t MUT uint8
+  -> output3:buffer_t MUT uint8
+  -> outputByteLen:size_t{v outputByteLen == length output0 /\ 
+                          v outputByteLen == length output1 /\
+                          v outputByteLen == length output2 /\
+                          v outputByteLen == length output3}
+  -> input0:buffer_t MUT uint8
+  -> input1:buffer_t MUT uint8
+  -> input2:buffer_t MUT uint8
+  -> input3:buffer_t MUT uint8
+  -> inputByteLen:size_t{v inputByteLen == length input0 /\ 
+                         v inputByteLen == length input1 /\
+                         v inputByteLen == length input2 /\
+                         v inputByteLen == length input3}
+  -> Stack unit
+     (requires fun h ->
+       live4 h (input0 <: lbuffer uint8 inputByteLen)
+               (input1 <: lbuffer uint8 inputByteLen)
+               (input2 <: lbuffer uint8 inputByteLen)
+               (input3 <: lbuffer uint8 inputByteLen) /\
+       live4 h (output0 <: lbuffer uint8 outputByteLen)
+               (output1 <: lbuffer uint8 outputByteLen)
+               (output2 <: lbuffer uint8 outputByteLen)
+               (output3 <: lbuffer uint8 outputByteLen) /\
+       internally_disjoint4 (output0 <: lbuffer uint8 outputByteLen)
+                            (output1 <: lbuffer uint8 outputByteLen)
+                            (output2 <: lbuffer uint8 outputByteLen)
+                            (output3 <: lbuffer uint8 outputByteLen))
+     (ensures  fun h0 _ h1 ->
+       modifies (loc output0 |+| loc output1 |+| loc output2 |+| loc output3) h0 h1 /\
+       as_seq h1 (output0 <: lbuffer uint8 outputByteLen) ==
+        S.shake256 (v inputByteLen) (as_seq h0 (input0 <: lbuffer uint8 inputByteLen)) (v outputByteLen) /\
+       as_seq h1 (output1 <: lbuffer uint8 outputByteLen) ==
+        S.shake256 (v inputByteLen) (as_seq h0 (input1 <: lbuffer uint8 inputByteLen)) (v outputByteLen) /\
+       as_seq h1 (output2 <: lbuffer uint8 outputByteLen) ==
+        S.shake256 (v inputByteLen) (as_seq h0 (input2 <: lbuffer uint8 inputByteLen)) (v outputByteLen) /\
+       as_seq h1 (output3 <: lbuffer uint8 outputByteLen) ==
+        S.shake256 (v inputByteLen) (as_seq h0 (input3 <: lbuffer uint8 inputByteLen)) (v outputByteLen))
+let shake256 output0 output1 output2 output3 outputByteLen
+      input0 input1 input2 input3 inputByteLen =
+  admit();
+  let ib = ntup4 (input0,(input1,(input2,input3))) in
+  let rb = ntup4 (output0,(output1,(output2,output3))) in
+  keccak #Shake256 #M256 1088ul (* 512ul *) inputByteLen ib (byte 0x1F) outputByteLen rb
+
+val sha3_224:
+  output0:lbuffer uint8 28ul
+  -> output1:lbuffer uint8 28ul
+  -> output2:lbuffer uint8 28ul
+  -> output3:lbuffer uint8 28ul
+  -> input0:buffer_t MUT uint8
+  -> input1:buffer_t MUT uint8
+  -> input2:buffer_t MUT uint8
+  -> input3:buffer_t MUT uint8
+  -> inputByteLen:size_t{v inputByteLen == length input0 /\ 
+                         v inputByteLen == length input1 /\
+                         v inputByteLen == length input2 /\
+                         v inputByteLen == length input3}
+  -> Stack unit
+     (requires fun h ->
+       live4 h (input0 <: lbuffer uint8 inputByteLen)
+               (input1 <: lbuffer uint8 inputByteLen)
+               (input2 <: lbuffer uint8 inputByteLen)
+               (input3 <: lbuffer uint8 inputByteLen) /\
+       live4 h output0 output1 output2 output3 /\
+       internally_disjoint4 output0 output1 output2 output3)
+     (ensures  fun h0 _ h1 ->
+       modifies (loc output0 |+| loc output1 |+| loc output2 |+| loc output3) h0 h1 /\
+       as_seq h1 output0 == S.sha3_224 (v inputByteLen) (as_seq h0 (input0 <: lbuffer uint8 inputByteLen)) /\
+       as_seq h1 output1 == S.sha3_224 (v inputByteLen) (as_seq h0 (input1 <: lbuffer uint8 inputByteLen)) /\
+       as_seq h1 output2 == S.sha3_224 (v inputByteLen) (as_seq h0 (input2 <: lbuffer uint8 inputByteLen)) /\
+       as_seq h1 output3 == S.sha3_224 (v inputByteLen) (as_seq h0 (input3 <: lbuffer uint8 inputByteLen)))
+let sha3_224 output0 output1 output2 output3
+        input0 input1 input2 input3 inputByteLen =
+  admit();
+  let ib = ntup4 (input0,(input1,(input2,input3))) in
+  let rb = ntup4 (output0,(output1,(output2,output3))) in
+  keccak #SHA3_224 #M256 1152ul (* 448ul *) inputByteLen ib (byte 0x06) 28ul rb
+
+val sha3_256:
+  output0:lbuffer uint8 32ul
+  -> output1:lbuffer uint8 32ul
+  -> output2:lbuffer uint8 32ul
+  -> output3:lbuffer uint8 32ul
+  -> input0:buffer_t MUT uint8
+  -> input1:buffer_t MUT uint8
+  -> input2:buffer_t MUT uint8
+  -> input3:buffer_t MUT uint8
+  -> inputByteLen:size_t{v inputByteLen == length input0 /\ 
+                         v inputByteLen == length input1 /\
+                         v inputByteLen == length input2 /\
+                         v inputByteLen == length input3}
+  -> Stack unit
+     (requires fun h ->
+       live4 h (input0 <: lbuffer uint8 inputByteLen)
+               (input1 <: lbuffer uint8 inputByteLen)
+               (input2 <: lbuffer uint8 inputByteLen)
+               (input3 <: lbuffer uint8 inputByteLen) /\
+       live4 h output0 output1 output2 output3 /\
+       internally_disjoint4 output0 output1 output2 output3)
+     (ensures  fun h0 _ h1 ->
+       modifies (loc output0 |+| loc output1 |+| loc output2 |+| loc output3) h0 h1 /\
+       as_seq h1 output0 == S.sha3_256 (v inputByteLen) (as_seq h0 (input0 <: lbuffer uint8 inputByteLen)) /\
+       as_seq h1 output1 == S.sha3_256 (v inputByteLen) (as_seq h0 (input1 <: lbuffer uint8 inputByteLen)) /\
+       as_seq h1 output2 == S.sha3_256 (v inputByteLen) (as_seq h0 (input2 <: lbuffer uint8 inputByteLen)) /\
+       as_seq h1 output3 == S.sha3_256 (v inputByteLen) (as_seq h0 (input3 <: lbuffer uint8 inputByteLen)))
+let sha3_256 output0 output1 output2 output3
+        input0 input1 input2 input3 inputByteLen =
+  admit();
+  let ib = ntup4 (input0,(input1,(input2,input3))) in
+  let rb = ntup4 (output0,(output1,(output2,output3))) in
+  keccak #SHA3_256 #M256 1088ul (* 512ul *) inputByteLen ib (byte 0x06) 32ul rb
+
+val sha3_384:
+  output0:lbuffer uint8 48ul
+  -> output1:lbuffer uint8 48ul
+  -> output2:lbuffer uint8 48ul
+  -> output3:lbuffer uint8 48ul
+  -> input0:buffer_t MUT uint8
+  -> input1:buffer_t MUT uint8
+  -> input2:buffer_t MUT uint8
+  -> input3:buffer_t MUT uint8
+  -> inputByteLen:size_t{v inputByteLen == length input0 /\ 
+                         v inputByteLen == length input1 /\
+                         v inputByteLen == length input2 /\
+                         v inputByteLen == length input3}
+  -> Stack unit
+     (requires fun h ->
+       live4 h (input0 <: lbuffer uint8 inputByteLen)
+               (input1 <: lbuffer uint8 inputByteLen)
+               (input2 <: lbuffer uint8 inputByteLen)
+               (input3 <: lbuffer uint8 inputByteLen) /\
+       live4 h output0 output1 output2 output3 /\
+       internally_disjoint4 output0 output1 output2 output3)
+     (ensures  fun h0 _ h1 ->
+       modifies (loc output0 |+| loc output1 |+| loc output2 |+| loc output3) h0 h1 /\
+       as_seq h1 output0 == S.sha3_384 (v inputByteLen) (as_seq h0 (input0 <: lbuffer uint8 inputByteLen)) /\
+       as_seq h1 output1 == S.sha3_384 (v inputByteLen) (as_seq h0 (input1 <: lbuffer uint8 inputByteLen)) /\
+       as_seq h1 output2 == S.sha3_384 (v inputByteLen) (as_seq h0 (input2 <: lbuffer uint8 inputByteLen)) /\
+       as_seq h1 output3 == S.sha3_384 (v inputByteLen) (as_seq h0 (input3 <: lbuffer uint8 inputByteLen)))
+let sha3_384 output0 output1 output2 output3
+        input0 input1 input2 input3 inputByteLen =
+  admit();
+  let ib = ntup4 (input0,(input1,(input2,input3))) in
+  let rb = ntup4 (output0,(output1,(output2,output3))) in
+  keccak #SHA3_384 #M256 832ul (* 768ul *) inputByteLen ib (byte 0x06) 48ul rb
+
+val sha3_512:
+  output0:lbuffer uint8 64ul
+  -> output1:lbuffer uint8 64ul
+  -> output2:lbuffer uint8 64ul
+  -> output3:lbuffer uint8 64ul
+  -> input0:buffer_t MUT uint8
+  -> input1:buffer_t MUT uint8
+  -> input2:buffer_t MUT uint8
+  -> input3:buffer_t MUT uint8
+  -> inputByteLen:size_t{v inputByteLen == length input0 /\ 
+                         v inputByteLen == length input1 /\
+                         v inputByteLen == length input2 /\
+                         v inputByteLen == length input3}
+  -> Stack unit
+     (requires fun h ->
+       live4 h (input0 <: lbuffer uint8 inputByteLen)
+               (input1 <: lbuffer uint8 inputByteLen)
+               (input2 <: lbuffer uint8 inputByteLen)
+               (input3 <: lbuffer uint8 inputByteLen) /\
+       live4 h output0 output1 output2 output3 /\
+       internally_disjoint4 output0 output1 output2 output3)
+     (ensures  fun h0 _ h1 ->
+       modifies (loc output0 |+| loc output1 |+| loc output2 |+| loc output3) h0 h1 /\
+       as_seq h1 output0 == S.sha3_512 (v inputByteLen) (as_seq h0 (input0 <: lbuffer uint8 inputByteLen)) /\
+       as_seq h1 output1 == S.sha3_512 (v inputByteLen) (as_seq h0 (input1 <: lbuffer uint8 inputByteLen)) /\
+       as_seq h1 output2 == S.sha3_512 (v inputByteLen) (as_seq h0 (input2 <: lbuffer uint8 inputByteLen)) /\
+       as_seq h1 output3 == S.sha3_512 (v inputByteLen) (as_seq h0 (input3 <: lbuffer uint8 inputByteLen)))
+let sha3_512 output0 output1 output2 output3
+        input0 input1 input2 input3 inputByteLen =
+  admit();
+  let ib = ntup4 (input0,(input1,(input2,input3))) in
+  let rb = ntup4 (output0,(output1,(output2,output3))) in
+  keccak #SHA3_512 #M256 576ul (* 1024ul *) inputByteLen ib (byte 0x06) 64ul rb
