Makefile
@@ -659,7 +659,6 @@ REQUIRED_FLAGS	= \
 
 TARGET_H_INCLUDE = -add-early-include '"krml/internal/target.h"'
 
-
 # Note: we include libintvector.h in C files whenever possible, but fall back to
 # including this header in .h when the public API of a given algorithm (e.g.
 # Poly1305/256) directly refers to a LibIntVector type.
@@ -682,7 +681,9 @@ INTRINSIC_FLAGS = \
   -add-include 'Hacl_SHA2_Vec256.c:"libintvector.h"' \
   \
   -add-include 'Hacl_Hash_Blake2b_256:"libintvector.h"' \
-  -add-include 'Hacl_Poly1305_256:"libintvector.h"'
+  -add-include 'Hacl_Poly1305_256:"libintvector.h"' \
+  \
+  -add-include 'Hacl_Hash_SHA3_Simd256.c:"libintvector.h"'
 
 # Disabled for distributions that don't include code based on intrinsics.
 INTRINSIC_INT_FLAGS = \
@@ -721,7 +722,8 @@ LEGACY_BUNDLE = -bundle EverCrypt[rename=EverCrypt_Legacy]
 BUNDLE_FLAGS	=\
   $(BLAKE2_BUNDLE) \
   $(SHA3_BUNDLE) \
-  $(SHA3_VEC_BUNDLE) \
+  $(SHA3_SCALAR_BUNDLE) \
+  $(SHA3_SIMD256_BUNDLE) \
   $(HASH_BUNDLE) \
   $(E_HASH_BUNDLE) \
   $(SHA2MB_BUNDLE) \
@@ -865,7 +867,6 @@ dist/%/Makefile.basic: $(ALL_KRML_FILES) dist/LICENSE.txt $(HAND_WRITTEN_FILES) 
 	  -fparentheses \
 	  -fcast-allocations \
 	  -fextern-c \
-	  -dinline -dreachability \
 	  $(notdir $(HAND_WRITTEN_FILES)) \
 	  -o libevercrypt.a
 	echo "This code was generated with the following toolchain." > $(dir $@)/INFO.txt
@@ -889,7 +890,6 @@ dist/test/c/%.c: $(ALL_KRML_FILES)
 	  -header $(HACL_HOME)/dist/LICENSE.txt \
 	  -no-prefix $(subst _,.,$*) \
           -library Hacl.P256,Hacl.K256.*,Hacl.Impl.*,EverCrypt.* \
-	  -add-include '"krml/internal/compat.h"' \
 	  -add-include '"internal/Hacl_Hash_SHA2.h"' \
 	  -static-header Hacl.Impl.SHA2.Generic \
 	  -fparentheses -fcurly-braces -fno-shadow \
